\chapter{Linear Transformations}

\section{Linear Transformations}

\Exercise1 Which of the following functions $T$ from $R^2$ into $R^2$
are linear transformations?
\begin{enumerate}
\item $T(x_1, x_2) = (1 + x_1, x_2)$;
  \begin{solution}
    $T$ cannot be a linear transformation since
    \begin{equation*}
      T(0, 0) = (1, 0) \neq (0, 0). \qedhere
    \end{equation*}
  \end{solution}
\item $T(x_1, x_2) = (x_2, x_1)$;
  \begin{solution}
    $T$ is a linear transformation: let $c$ be a scalar and let
    $\alpha = (x_1, x_2)$ and $\beta = (y_1, y_2)$. Then
    \begin{align*}
      T(c\alpha + \beta)
      &= T(cx_1 + y_1, cx_2 + y_2) \\
      &= (cx_2 + y_2, cx_1 + y_1) \\
      &= c(x_2, x_1) + (y_2, y_1) \\
      &= cT(\alpha) + T(\beta). \qedhere
    \end{align*}
  \end{solution}
\item $T(x_1, x_2) = (x_1^2, x_2)$;
  \begin{solution}
    $T$ is not a linear transformation. For example,
    \begin{equation*}
      T(1, 0) + T(2, 0) = (1, 0) + (4, 0) = (5, 0)
    \end{equation*}
    but
    \begin{equation*}
      T((1, 0) + (2, 0)) = T(3, 0) = (9, 0). \qedhere
    \end{equation*}
  \end{solution}
\item $T(x_1, x_2) = (\sin x_1, x_2)$;
  \begin{solution}
    $T$ is not a linear transformation since
    \begin{equation*}
      T\left(\frac\pi2, 0\right) + T\left(\frac\pi2, 0\right)
      = (1, 0) + (1, 0) = (2, 0)
    \end{equation*}
    while
    \begin{equation*}
      T\left(\left(\frac\pi2, 0\right) + \left(\frac\pi2, 0\right)\right)
      = T(\pi, 0) = (0, 0). \qedhere
    \end{equation*}
  \end{solution}
\item $T(x_1, x_2) = (x_1 - x_2, 0)$.
  \begin{solution}
    Let $\alpha = (x_1, x_2)$ and $\beta = (y_1, y_2)$. Since
    \begin{align*}
      cT(\alpha) + T(\beta)
      &= c(x_1 - x_2, 0) + (y_1 - y_2, 0) \\
      &= (cx_1 - cx_2 + y_1 - y_2, 0) \\
      &= ((cx_1 + y_1) - (cx_2 + y_2), 0) \\
      &= T(cx_1 + y_1, cx_2 + y_2) \\
      &= T(c\alpha + \beta),
    \end{align*}
    we see that $T$ is a linear transformation.
  \end{solution}
\end{enumerate}

\Exercise2 Find the range, rank, null space, and nullity for the zero
transformation and the identity transformation on a finite-dimensional
space $V$.
\begin{solution}
  Let $V$ be a vector space of finite dimension $n$, let
  $T\colon V\to V$ be the zero transformation, and let
  $U\colon V\to V$ be the identity transformation.

  Then the range of $T$ is clearly the set consisting of the zero
  vector alone, and the null space is $V$ itself. The rank of $T$ is
  then $0$ (the zero subspace has the empty set as a basis) and the
  nullity of $T$ is $n$.

  For the identity transformation $U$, we see that the range is all of
  $V$, while the null space is the zero subspace $\{0\}$. Then the
  rank of $U$ is $n$ and the nullity of $U$ is $0$.

  Note that in each case, the rank plus the nullity is $n$, in
  agreement with Theorem~2.
\end{solution}

\Exercise3 Describe the range and the null space for the
differentiation transformation of Example~2. Do the same for the
integration transformation of Example~5.
\begin{solution}
  Let $V$ be the space of polynomial functions from $F$ into $F$ and
  let $D$ be the differentiation transformation. Given a polynomial
  \begin{equation*}
    f(x) = c_0 + c_1x + \cdots + c_kx^k,
  \end{equation*}
  we can always find another polynomial $g(x)$ such that
  $(Dg)(x) = f(x)$, namely the polynomial
  \begin{equation*}
    g(x) = c_0x + \frac12c_1x^2 + \cdots + \frac1{k+1}c_kx^{k+1}.
  \end{equation*}
  Therefore the range of $D$ is $V$.

  A function $f$ has zero derivative if and only if $f$ is constant,
  \begin{equation*}
    f(x) = c_0, \quad \text{for some $c_0$ in $F$.}
  \end{equation*}
  So the null space of $D$ is the space of constant functions.

  Now, let $T$ be the integration transformation defined in
  Example~5. We can integrate any polynomial to get another
  polynomial, but because of the manner in which $T$ was defined, the
  resulting polynomial will always have a constant term of $0$. Let
  $f$ be a polynomial with constant term zero,
  \begin{equation*}
    f(x) = c_1x + c_2x^2 + \cdots + c_kx^k.
  \end{equation*}
  Then the function $g(x) = (Df)(x)$ is such that $(Tg)(x) = f(x)$. So
  we see that the range of $T$ is the space of polynomials with zero
  constant term.

  Lastly, if $f$ is a polynomial such that $(Tf)(x) = 0$, then $f$
  must be the zero polynomial. The null space of $T$ is therefore the
  trivial subspace $\{0\}$.
\end{solution}

\Exercise4 Is there a linear transformation $T$ from $R^3$ into $R^2$
such that $T(1, -1, 1) = (1, 0)$ and $T(1, 1, 1) = (0, 1)$?
\begin{solution}
  Yes. In fact, there are infinitely many such transformations, as we
  will now show.

  Let $\alpha = (1, -1, 1)$ and let $\beta = (1, 1, 1)$. Since neither
  $\alpha$ nor $\beta$ is a multiple of the other, the set
  $\{\alpha, \beta\}$ is linearly independent. Therefore it can be
  extended to a basis for $R^3$. The existence of a linear
  transformation $T$ such that $T(\alpha) = (1, 0)$ and
  $T(\beta) = (0, 1)$ now follows from Theorem~1.

  To find such a transformation explicitly, we will form a basis for
  $R^3$. If we let $\gamma = (1, 0, 0)$, for example, it is not
  difficult to show that $\{\alpha, \beta, \gamma\}$ is a linearly
  independent set of vectors which spans $R^3$.

  We want to be able to write a vector $\rho = (b_1, b_2, b_3)$ as a
  linear combination of $\alpha$, $\beta$, and $\gamma$. To do this,
  we will set up an augmented matrix and perform row-reduction, as we
  have done before in Chapter~2:
  \begin{equation*}
    \begin{bmatrix}
      1 & 1 & 1 & y_1 \\
      -1 & 1 & 0 & y_2 \\
      1 & 1 & 0 & y_3
    \end{bmatrix}
    \rightarrow
    \begin{bmatrix}
      1 & 0 & 0 & \frac12y_3 - \frac12y_2 \\[3pt]
      0 & 1 & 0 & \frac12y_2 + \frac12y_3 \\[3pt]
      0 & 0 & 1 & y_1 - y_3
    \end{bmatrix}.
  \end{equation*}
  So we may write
  \begin{equation*}
    \rho = (b_1, b_2, b_3) =
    \frac12(b_3 - b_2)\alpha + \frac12(b_2 + b_3)\beta
    + (b_1 - b_3)\gamma.
  \end{equation*}

  Now suppose the transformation $T$ is such that
  $T(\gamma) = (x_1, x_2)$, for some $x_1$ and $x_2$ in $R$. Then we
  have
  \begin{align*}
    T(b_1, b_2, b_3)
    &= T\left(\frac12(b_3 - b_2)\alpha + \frac12(b_2 + b_3)\beta
      + (b_1 - b_3)\gamma\right) \\[3pt]
    &= \frac12(b_3 - b_2)T(\alpha) + \frac12(b_2 + b_3)T(\beta)
      + (b_1 - b_3)T(\gamma) \\[3pt]
    &= \frac12(b_3 - b_2, 0) + \frac12(0, b_2 + b_3)
      + (x_1b_1 - x_1b_3, x_2b_1 - x_2b_3) \\[3pt]
    &= \frac12(2x_1b_1 - b_2 + (1 - 2x_1)b_3,
      2x_2b_1 + b_2 + (1 - 2x_2)b_3).
  \end{align*}

  So, for example, taking
  $(x_1, x_2) = \left(\frac12, \frac12\right)$, we get
  \begin{equation*}
    T(b_1, b_2, b_3) = \left(\frac12b_1 - \frac12b_2,
      \frac12b_1 + \frac12b_2\right).
  \end{equation*}
  By picking different values for $x_1$ and $x_2$, we see that there
  are infinitely many possibilities for $T$.
\end{solution}
