\section{The Transpose of a Linear Transformation}

\Exercise1 Let $F$ be a field and let $f$ be the linear functional on
$F^2$ defined by
\begin{equation*}
  f(x_1,x_2) = ax_1 + bx_2.
\end{equation*}
For each of the following linear operators $T$, let $g = T^tf$, and
find $g(x_1,x_2)$.
\begin{enumerate}
\item $T(x_1,x_2) = (x_1,0)$
  \begin{solution}
    We have
    \begin{align*}
      g(x_1,x_2)
      &= (T^tf)(x_1,x_2) \\
      &= f(T(x_1,x_2)) \\
      &= f(x_1,0) \\
      &= ax_1. \qedhere
    \end{align*}
  \end{solution}

\item $T(x_1,x_2) = (-x_2,x_1)$
  \begin{solution}
    In this case, we get
    \begin{align*}
      g(x_1,x_2)
      &= f(T(x_1,x_2)) \\
      &= f(-x_2,x_1) \\
      &= -ax_2 + bx_1. \qedhere
    \end{align*}
  \end{solution}

\item $T(x_1,x_2) = (x_1 - x_2, x_1 + x_2)$
  \begin{solution}
    \begin{align*}
      g(x_1,x_2)
      &= f(x_1 - x_2, x_1 + x_2) \\
      &= (b + a)x_1 + (b - a)x_2. \qedhere
    \end{align*}
  \end{solution}
\end{enumerate}
